elim_exists soundness

pulse/examples/dsls/mini_steel/Pulse.Soundness.Exists.fst
@@ -1,3 +1,4 @@
 module Pulse.Soundness.Exists
 
+let exists_inversion _ = admit ()
 let elim_exists_soundness _ _ = admit ()
