pulse/examples/dsls/mini_steel/Pulse.Soundness.Exists.fsti
@@ -3,25 +3,41 @@ module Pulse.Soundness.Exists
 open FStar.Reflection
 open Refl.Typing
 open Pulse.Elaborate.Pure
+open Pulse.Typing
+open Pulse.Soundness.Common
+
+val exists_inversion
+  (#f:stt_env)
+  (#g:env)
+  (#u:universe)
+  (#a:term)
+  (#p:term)
+  (e_typing:typing (extend_env_l f g)
+                   (mk_exists u a p)
+                   vprop_tm)
+
+  : GTot (typing (extend_env_l f g) p
+                 (mk_arrow (a, Q_Explicit) vprop_tm))
 
 (*
 
  g |- a : Type u
- g |- fun _ -> p : a -> vprop
- --------------------------------------------------------------------------------------------------
- g |- elim_exists<u> a (fun _ -> p) : stt_ghost<u> a emp (exists_<u> (fun _ -> p)) (fun _ -> p)
+ g |- p : a -> vprop
+ ----------------------------------------------------------------
+ g |- elim_exists<u> a p : stt_ghost<u> a emp (exists_<u> p) p
 
 *)
 
 val elim_exists_soundness
-  (#g:fstar_top_env)
+  (#f:stt_env)
+  (#g:env)
   (#u:universe)
   (#a:term)
   (#p:term)
-  (a_typing:typing g a (pack_ln (Tv_Type u)))
-  (p_typing:typing g (mk_abs a Q_Explicit p)
-                     (mk_arrow (a, Q_Explicit) vprop_tm))
+  (a_typing:typing (extend_env_l f g) a (pack_ln (Tv_Type u)))
+  (p_typing:typing (extend_env_l f g) p (mk_arrow (a, Q_Explicit) vprop_tm))
 
-  : GTot (typing g (mk_elim_exists u a p) (mk_stt_ghost_comp u a emp_inames_tm
-                                             (mk_exists u a p)
-                                             (mk_abs a Q_Explicit p)))
+  : GTot (typing (extend_env_l f g)
+                 (mk_elim_exists u a p)
+                 (mk_stt_ghost_comp u a emp_inames_tm
+                    (mk_exists u a p) p))
